Lean4Lean/Verify/Environment.lean
@@ -1,0 +1,34 @@
+import Lean4Lean.Verify.LocalContext
+import Lean4Lean.Theory.Typing.Env
+
+namespace Lean4Lean
+open Lean
+
+def isAsSafeAs : DefinitionSafety → ConstantInfo → Bool
+  | .unsafe, _ => true
+  | .partial, ci => !ci.isUnsafe
+  | .safe, ci => !ci.isUnsafe && !ci.isPartial
+
+variable (safety : DefinitionSafety) (ci : ConstantInfo) in
+inductive TrConstant : Option VConstant → Prop where
+  | safe : isAsSafeAs safety ci →
+    ci.levelParams.length = ci'.uvars →
+    TrExpr ci.levelParams [] ci.type ci'.type →
+    TrConstant (some ci')
+  | «unsafe» : ¬isAsSafeAs safety ci → TrConstant none
+
+def TrRecDefEq : RecursorVal → RecursorRule → VDefEq → Prop := sorry
+
+def TrDefEq : ConstantInfo → VDefEq → Prop
+  | .defnInfo ci, df => ∃ ty' val',
+    TrExpr ci.levelParams [] ci.type ty' ∧
+    TrExpr ci.levelParams [] ci.value val' ∧
+    df = VDefVal.toDefEq ⟨⟨⟨ci.levelParams.length, ty'⟩, ci.name⟩, val'⟩
+  | .quotInfo _, df => df = quotDefEq
+  | .recInfo ci, df => ∃ rule ∈ ci.rules, TrRecDefEq ci rule df
+  | _, _ => False
+
+structure TrEnv (safety : DefinitionSafety) (env : Environment) (venv : VEnv) : Prop where
+  constants : env.find? n = some ci →
+    ∃ ci', TrConstant safety ci ci' ∧ venv.constants n = some ci'
+  defeqs : venv.defeqs df ↔ ∃ ci, isAsSafeAs safety ci ∧ TrDefEq ci df
