Lean4Lean/Verify/TypeChecker/Basic.lean
@@ -1,0 +1,3 @@
+import Lean4Lean.Verify.Environment
+
+namespace Lean4Lean
